WIP

src/NoSync2Stutter.v
@@ -721,9 +721,9 @@ Section GENORDER.
   Variable state_tgt: Type.
 
   Variable _ident_src: ID.
-  Definition ident_src := sum_tid _ident_src.
+  Let ident_src := @ident_src _ident_src.
   Variable _ident_tgt: ID.
-  Definition ident_tgt := sum_tid _ident_tgt.
+  Let ident_tgt := @ident_tgt _ident_tgt.
 
   Variable wf_src: WF.
   Variable wf_tgt: WF.
@@ -1140,9 +1140,9 @@ Section PROOF.
   Variable state_tgt: Type.
 
   Variable _ident_src: ID.
-  Definition ident_src := sum_tid _ident_src.
+  Let ident_src := @ident_src _ident_src.
   Variable _ident_tgt: ID.
-  Definition ident_tgt := sum_tid _ident_tgt.
+  Let ident_tgt := @ident_tgt _ident_tgt.
 
   Variable wf_src: WF.
   Variable wf_tgt: WF.
@@ -1166,11 +1166,13 @@ Section PROOF.
           wf_stt tid
           R0 R1 (LRR: R0 -> R1 -> URA.car -> shared_rel)
           ps pt r_ctx src tgt (shr: shared) o0 o1
-          (LT: wf_stt.(lt) o0 o1)
+          (LE: wf_stt.(le) o0 o1)
           (LSIM: ModSimStutter.lsim wf_stt I tid LRR ps pt r_ctx (o0, src) tgt shr)
     :
     ModSimStutter.lsim wf_stt I tid LRR ps pt r_ctx (o1, src) tgt shr.
   Proof.
+    destruct LE as [EQ | LT].
+    { clarify. }
     revert_until tid. pcofix CIH; i.
     remember (o0, src) as osrc.
     move LSIM before CIH. revert_until LSIM.
@@ -1248,9 +1250,21 @@ Section PROOF.
 
   Qed.
 
-
   Let A R0 R1 := (bool * bool * URA.car * (itree srcE R0) * (itree tgtE R1) * shared)%type.
-  Let wf_stt {R0 R1} := (@ord_tree_WF (A R0 R1)).
+  Let wf_ot {R0 R1} := @ord_tree_WF (A R0 R1).
+  Let wf_stt {R0 R1} := sum_WF (sum_WF (@wf_ot R0 R1) (@wf_ot R0 R1)) (@wf_ot R0 R1).
+
+  Definition mk_o {R0 R1}
+             (o: (@wf_ot R0 R1).(T)) (ps: bool) (itr_src: itree srcE R0): (@wf_stt R0 R1).(T) :=
+    if ps
+    then match (observe itr_src) with
+         | VisF ((|Yield)|)%sum _ => (inl (inr o))
+         | _ => (inr (@ord_tree_base _))
+         end
+    else match (observe itr_src) with
+         | VisF ((|Yield)|)%sum _ => (inl (inl o))
+         | _ => (inr (@ord_tree_base _))
+         end.
 
   Lemma nosync_implies_stutter
         tid
@@ -1260,133 +1274,148 @@ Section PROOF.
         (LSIM: ModSimNoSync.lsim I tid LRR ps pt r_ctx src tgt shr)
     :
     exists (o: (@wf_stt R0 R1).(T)),
-      ModSimStutter.lsim wf_stt I tid LRR ps pt r_ctx (o, src) tgt shr.
+      ModSimStutter.lsim (@wf_stt R0 R1) I tid LRR ps pt r_ctx (o, src) tgt shr.
   Proof.
-    punfold LSIM.
-    pattern R0, R1, LRR, ps, pt, r_ctx, src, tgt, shr.
-    revert R0 R1 LRR ps pt r_ctx src tgt shr LSIM. apply pind9_acc.
-    intros rr DEC IH. clear DEC. intros R0 R1 LRR ps pt r_ctx src tgt shr LSIM.
-    eapply pind9_unfold in LSIM.
-    2:{ eapply ModSimNoSync._lsim_mon. }
+    eapply nosync_geno in LSIM. des. exists (mk_o o ps src).
+    (* revert_until tid. *)
+    (* ginit. gcofix CIH. i. *)
+
+    remember (o, src) as osrc.
+    move LSIM before tid. revert_until LSIM.
+    (* move LSIM before CIH. revert_until LSIM. *)
+    pattern R0, R1, LRR, ps, pt, r_ctx, osrc, tgt, shr.
+    revert R0 R1 LRR ps pt r_ctx osrc tgt shr LSIM. apply pind9_acc.
+    intros rr DEC IH. clear DEC. intros R0 R1 LRR ps pt r_ctx osrc tgt shr LSIM.
+    intros src o Eosrc. clarify.
+    eapply pind9_unfold in LSIM; eauto with paco.
     inv LSIM.
 
-    { remember (fun _: (A R0 R1) => @ord_tree_base (A R0 R1)) as ao. exists (ord_tree_cons ao).
-      pfold. eapply pind9_fold. econs 1; eauto.
-      instantiate (1:=ao (ps, pt, r_ctx, Ret r_src, Ret r_tgt, (ths, im_src, im_tgt, st_src, st_tgt, r_shared))).
-      eapply ord_tree_lt_intro.
+    { unfold mk_o. des_ifs.
+      - pfold. eapply pind9_fold. econs 1; eauto.
+        instantiate (1:=inl (inl o1)). ss. econs 3.
+      - pfold. eapply pind9_fold. econs 1; eauto.
+        instantiate (1:=inl (inl o1)). ss. econs 3.
     }
 
-    { destruct LSIM0 as [LSIM IND]. eapply IH in IND. des. exists o.
+    { destruct GENO as [GENO IND]. eapply IH in IND; eauto.
       pfold. eapply pind9_fold. econs 2; eauto.
-      split; ss. punfold IND.
+      split; ss.
+      eapply stutter_ord_weak in IND. punfold IND.
+      unfold mk_o. des_ifs; try reflexivity.
+      - right. ss. econs 3.
+      - right. ss. econs 3.
     }
-    { des. destruct LSIM0 as [LSIM IND]. eapply IH in IND. des. exists o.
+    { des. destruct GENO as [GENO IND]. eapply IH in IND; eauto.
       pfold. eapply pind9_fold. econs 3; eauto. exists x.
-      split; ss. punfold IND.
+      split; ss.
+      eapply stutter_ord_weak in IND. punfold IND.
+      unfold mk_o. des_ifs; try reflexivity.
+      - right. ss. econs 3.
+      - right. ss. econs 3.
     }
-    { destruct LSIM0 as [LSIM IND]. eapply IH in IND. des. exists o.
+    { destruct GENO as [GENO IND]. eapply IH in IND; eauto.
       pfold. eapply pind9_fold. econs 4; eauto.
-      split; ss. punfold IND.
+      split; ss.
+      eapply stutter_ord_weak in IND. punfold IND.
+      unfold mk_o. des_ifs; try reflexivity.
+      - right. ss. econs 3.
+      - right. ss. econs 3.
     }
-    { destruct LSIM0 as [LSIM IND]. eapply IH in IND. des. exists o.
+    { destruct GENO as [GENO IND]. eapply IH in IND; eauto.
       pfold. eapply pind9_fold. econs 5; eauto.
-      split; ss. punfold IND.
+      split; ss.
+      eapply stutter_ord_weak in IND. punfold IND.
+      unfold mk_o. des_ifs; try reflexivity.
+      - right. ss. econs 3.
+      - right. ss. econs 3.
     }
-    { destruct LSIM0 as [LSIM IND]. eapply IH in IND. des. exists o.
+    { destruct GENO as [GENO IND]. eapply IH in IND; eauto.
       pfold. eapply pind9_fold. econs 6; eauto.
-      split; ss. punfold IND.
+      split; ss.
+      eapply stutter_ord_weak in IND. punfold IND.
+      unfold mk_o. des_ifs; try reflexivity.
+      - right. ss. econs 3.
+      - right. ss. econs 3.
     }
-    { exists (@ord_tree_base (A R0 R1)).
-      pfold. eapply pind9_fold. econs 7; eauto.
-    }
-    { des. destruct LSIM as [LSIM IND]. eapply IH in IND. des. exists o.
+    { pfold. eapply pind9_fold. econs 7; eauto. }
+    { des. destruct GENO0 as [GENO IND]. eapply IH in IND; eauto.
       pfold. eapply pind9_fold. econs 8; eauto. esplits; eauto.
-      split; ss. punfold IND.
+      split; ss.
+      eapply stutter_ord_weak in IND. punfold IND.
+      unfold mk_o. des_ifs; try reflexivity.
+      - right. ss. econs 3.
+      - right. ss. econs 3.
     }
 
-    { destruct LSIM0 as [LSIM IND]. eapply IH in IND. des. exists o.
+    { destruct GENO as [GENO IND]. eapply IH in IND; eauto.
       pfold. eapply pind9_fold. econs 9; eauto.
-      split; ss. punfold IND.
-    }
-
-    { hexploit ord_tree_join.
-      { instantiate (2:=A R0 R1).
-        instantiate (2:= fun '(ps, pt, rs, src, tgt, shr) => @rr R0 R1 LRR ps pt rs src tgt shr).
-        i. ss. des_ifs. eapply IH in SAT.
-        instantiate (1:= fun '(ps, pt, rs, src, tgt, shr) o => lsim wf_stt I tid LRR ps pt rs (o, src) tgt shr).
-        eauto.
-      }
-      intro JOIN. des. exists o1. pfold. eapply pind9_fold. econs 10. i. specialize (LSIM0 x).
-      destruct LSIM0 as [LSIM IND].
-      specialize (JOIN (ps, true, r_ctx, src, (ktr_tgt x), (ths, im_src, im_tgt, st_src, st_tgt, r_shared))). des_ifs.
-      eapply JOIN in IND; clear JOIN. des.
       split; ss.
-      eapply stutter_ord_weak in IND. punfold IND. auto.
+      eapply stutter_ord_weak in IND. punfold IND.
+      left; auto.
     }
-
-    { destruct LSIM0 as [LSIM IND]. eapply IH in IND. des. exists o.
+    { pfold. eapply pind9_fold. econs 10; eauto. i. specialize (GENO x).
+      destruct GENO as [GENO IND]. eapply IH in IND; eauto.
+      split; ss.
+      eapply stutter_ord_weak in IND. punfold IND.
+      left; auto.
+    }
+    { destruct GENO as [GENO IND]. eapply IH in IND; eauto.
       pfold. eapply pind9_fold. econs 11; eauto.
-      split; ss. punfold IND.
-    }
-    { destruct LSIM0 as [LSIM IND]. eapply IH in IND. des. exists o.
-      pfold. eapply pind9_fold. econs 12; eauto.
-      split; ss. punfold IND.
-    }
-    { destruct LSIM0 as [LSIM IND]. eapply IH in IND. des. exists o.
-      pfold. eapply pind9_fold. econs 13; eauto.
-      split; ss. punfold IND.
-    }
-
-    { hexploit ord_tree_join.
-      { instantiate (2:=A R0 R1).
-        instantiate (2:= fun '(ps, pt, rs, src, tgt, shr) => @rr R0 R1 LRR ps pt rs src tgt shr).
-        i. ss. des_ifs. eapply IH in SAT.
-        instantiate (1:= fun '(ps, pt, rs, src, tgt, shr) o => lsim wf_stt I tid LRR ps pt rs (o, src) tgt shr).
-        eauto.
-      }
-      intro JOIN. des. exists o1. pfold. eapply pind9_fold. econs 14. i. specialize (LSIM0 _ FAIR).
-      destruct LSIM0 as [LSIM IND].
-      specialize (JOIN (ps, true, r_ctx, src, (ktr_tgt ()), (ths, im_src, im_tgt1, st_src, st_tgt, r_shared))). des_ifs.
-      eapply JOIN in IND; clear JOIN. des.
       split; ss.
-      eapply stutter_ord_weak in IND. punfold IND. auto.
+      eapply stutter_ord_weak in IND. punfold IND.
+      left; auto.
+    }
+    { destruct GENO as [GENO IND]. eapply IH in IND; eauto.
+      pfold. eapply pind9_fold. econs 12; eauto.
+      split; ss.
+      eapply stutter_ord_weak in IND. punfold IND.
+      left; auto.
+    }
+    { destruct GENO as [GENO IND]. eapply IH in IND; eauto.
+      pfold. eapply pind9_fold. econs 13; eauto.
+      split; ss.
+      eapply stutter_ord_weak in IND. punfold IND.
+      left; auto.
+    }
+    { pfold. eapply pind9_fold. econs 14; eauto. i. specialize (GENO _ FAIR).
+      destruct GENO as [GENO IND]. eapply IH in IND; eauto.
+      split; ss.
+      eapply stutter_ord_weak in IND. punfold IND.
+      left; auto.
     }
 
-    { hexploit ord_tree_join.
-      { instantiate (2:=A R0 R1).
-        instantiate (2:= fun '(ps, pt, rs, src, tgt, shr) => @rr R0 R1 LRR ps pt rs src tgt shr).
-        i. ss. des_ifs. eapply IH in SAT.
-        instantiate (1:= fun '(ps, pt, rs, src, tgt, shr) o => lsim wf_stt I tid LRR ps pt rs (o, src) tgt shr).
-        eauto.
-      }
-      intro JOIN. des. exists o1. pfold. eapply pind9_fold. econs 15. i. specialize (LSIM0 ret).
-      destruct LSIM0 as [LSIM IND].
-      specialize (JOIN (true, true, r_ctx, ktr_src ret, ktr_tgt ret, (ths, im_src, im_tgt, st_src, st_tgt, r_shared))). des_ifs.
-      eapply JOIN in IND; clear JOIN. des.
-      eapply stutter_ord_weak in IND. punfold IND. auto.
+    { pfold. eapply pind9_fold. econs 15; eauto. i. specialize (GENO ret).
+      destruct GENO as [GENO IND]. eapply IH in IND; eauto.
+      eapply stutter_ord_weak in IND. punfold IND.
+      unfold mk_o. ss. des_ifs; try reflexivity.
+      - right. ss. econs 3.
+      - right. ss. econs 3.
     }
 
-    { hexploit ord_tree_join.
-      { instantiate (2:=A R0 R1).
-        instantiate (2:= fun '(ps, pt, rs, src, tgt, shr) => @rr R0 R1 LRR ps pt rs src tgt shr).
-        i. ss. des_ifs. eapply IH in SAT.
-        instantiate (1:= fun '(ps, pt, rs, src, tgt, shr) o => lsim wf_stt I tid LRR ps pt rs (o, src) tgt shr).
-        eauto.
-      }
-      intro JOIN. des. exists o1. pfold. eapply pind9_fold. econs 16; eauto. i.
-      specialize (LSIM0 _ _ _ _ _ _ _ INV0 VALID0 _ TGT).
-      destruct LSIM0 as [LSIM IND].
-      specialize (JOIN (ps, true, r_ctx1, (x <- trigger Yield;; ktr_src x), ktr_tgt (), (ths1, im_src1, im_tgt2, st_src1, st_tgt1, r_shared1))). des_ifs.
-      eapply JOIN in IND; clear JOIN. des. esplits; eauto.
-      split; ss. punfold IND.
+    { pfold. eapply pind9_fold. econs 16; eauto. i.
+      specialize (GENO _ _ _ _ _ _ _ INV0 VALID0 _ TGT). des.
+      destruct GENO0 as [GENO IND]. eapply IH in IND; eauto.
+      esplits. left. eapply ModSimStutter.lsim_reset_prog. eauto. 1,2: ss.
+      unfold mk_o; ss. rewrite !bind_trigger. ss.
+      des_ifs.
+      - econs 1. econs 2. auto.
+      - econs 1. econs 1. auto.
     }
 
-    { des. destruct LSIM as [LSIM IND]. eapply IH in IND. des. exists o.
+    { des. destruct GENO0 as [GENO IND]. eapply IH in IND; eauto.
       pfold. eapply pind9_fold. econs 17; eauto. esplits; eauto.
       split; ss. punfold IND.
     }
 
-    { exists (@ord_tree_base _). pfold. eapply pind9_fold. econs 18. pclearbot. auto. }
+    { eapply nosync_geno in GENO. des.
+      eapply stutter_ord_weak. instantiate (1:=mk_o o0 false src).
+      { ss. des_ifs; try reflexivity. right. ss. econs 1. econs 3. }
+      pfold. eapply pind9_fold. econs 18.
+      right.
+      (*TODO*)
+      eapply geno_ord_weak in GENO. instantiate (1:=mk_o o true src) in GENO.
+
+      pclearbot. auto. }
 
   Qed.
 
